ETCS_Ordinal_Inequalities.thy
@@ -2,7 +2,14 @@ theory ETCS_Ordinal_Inequalities
   imports ETCS_Exp ETCS_Comparison
 begin
 
-(*
+lemma exp_order_preserving_converse:
+  assumes a_type: "a \<in>\<^sub>c \<nat>\<^sub>c" and b_type: "b \<in>\<^sub>c \<nat>\<^sub>c" and c_type: "c \<in>\<^sub>c \<nat>\<^sub>c"
+  assumes "leq \<circ>\<^sub>c \<langle>a \<cdot>\<^sub>\<nat> (a ^\<^sub>\<nat> c) , b \<cdot>\<^sub>\<nat>(b ^\<^sub>\<nat> c)\<rangle> = \<t>"
+  assumes "c \<noteq> zero"
+  shows "leq \<circ>\<^sub>c \<langle>a , b\<rangle> = \<t>"
+  oops
+
+
 lemma exp_order_preserving1:
   assumes a_type: "a \<in>\<^sub>c \<nat>\<^sub>c" and b_type: "b \<in>\<^sub>c \<nat>\<^sub>c" and c_type: "c \<in>\<^sub>c \<nat>\<^sub>c"
   assumes leq: "leq \<circ>\<^sub>c \<langle>a , b\<rangle> = \<t>"
@@ -27,11 +34,168 @@ proof-
       by typecheck_cfuncs
     
     show "\<phi>\<^sup>\<sharp> \<circ>\<^sub>c zero = (\<t> \<circ>\<^sub>c \<beta>\<^bsub>(\<nat>\<^sub>c \<times>\<^sub>c \<nat>\<^sub>c) \<times>\<^sub>c \<nat>\<^sub>c\<^esub>)\<^sup>\<sharp> \<circ>\<^sub>c zero"
-    proof(rule same_evals_equal[where Z = one, where X = "\<Omega>", where A = "(\<nat>\<^sub>c \<times>\<^sub>c \<nat>\<^sub>c)\<times>\<^sub>cone"])
-      show "\<phi>\<^sup>\<sharp> \<circ>\<^sub>c zero \<in>\<^sub>c \<Omega>\<^bsup>((\<nat>\<^sub>c \<times>\<^sub>c \<nat>\<^sub>c) \<times>\<^sub>c one)\<^esup>" 
-        apply typecheck_cfuncs
-        oops
+    proof(rule same_evals_equal[where Z = one, where X = "\<Omega>", where A = "(\<nat>\<^sub>c \<times>\<^sub>c \<nat>\<^sub>c)"])
+      show phisharp_zero_type: "\<phi>\<^sup>\<sharp> \<circ>\<^sub>c zero \<in>\<^sub>c \<Omega>\<^bsup>(\<nat>\<^sub>c \<times>\<^sub>c \<nat>\<^sub>c)\<^esup>"
+        using \<phi>_sharp_type comp_type zero_type by auto
+      show "(\<t> \<circ>\<^sub>c \<beta>\<^bsub>(\<nat>\<^sub>c \<times>\<^sub>c \<nat>\<^sub>c) \<times>\<^sub>c \<nat>\<^sub>c\<^esub>)\<^sup>\<sharp> \<circ>\<^sub>c zero \<in>\<^sub>c \<Omega>\<^bsup>(\<nat>\<^sub>c \<times>\<^sub>c \<nat>\<^sub>c)\<^esup>"
+        using comp_type true_b_sharp_type zero_type by blast
+      show "eval_func \<Omega> (\<nat>\<^sub>c \<times>\<^sub>c \<nat>\<^sub>c) \<circ>\<^sub>c id\<^sub>c (\<nat>\<^sub>c \<times>\<^sub>c \<nat>\<^sub>c) \<times>\<^sub>f (\<phi>\<^sup>\<sharp> \<circ>\<^sub>c zero) =
+            eval_func \<Omega> (\<nat>\<^sub>c \<times>\<^sub>c \<nat>\<^sub>c) \<circ>\<^sub>c id\<^sub>c (\<nat>\<^sub>c \<times>\<^sub>c \<nat>\<^sub>c) \<times>\<^sub>f (\<t> \<circ>\<^sub>c \<beta>\<^bsub>(\<nat>\<^sub>c \<times>\<^sub>c \<nat>\<^sub>c) \<times>\<^sub>c \<nat>\<^sub>c\<^esub>)\<^sup>\<sharp> \<circ>\<^sub>c zero"
+      proof(rule one_separator[where X = "(\<nat>\<^sub>c \<times>\<^sub>c \<nat>\<^sub>c)\<times>\<^sub>c one", where Y="\<Omega>"])
+        show "eval_func \<Omega> (\<nat>\<^sub>c \<times>\<^sub>c \<nat>\<^sub>c) \<circ>\<^sub>c id\<^sub>c (\<nat>\<^sub>c \<times>\<^sub>c \<nat>\<^sub>c) \<times>\<^sub>f \<phi>\<^sup>\<sharp> \<circ>\<^sub>c zero : (\<nat>\<^sub>c \<times>\<^sub>c \<nat>\<^sub>c) \<times>\<^sub>c one \<rightarrow> \<Omega>"
+          by (typecheck_cfuncs, simp add: phisharp_zero_type)
+        show "eval_func \<Omega> (\<nat>\<^sub>c \<times>\<^sub>c \<nat>\<^sub>c) \<circ>\<^sub>c id\<^sub>c (\<nat>\<^sub>c \<times>\<^sub>c \<nat>\<^sub>c) \<times>\<^sub>f (\<t> \<circ>\<^sub>c \<beta>\<^bsub>(\<nat>\<^sub>c \<times>\<^sub>c \<nat>\<^sub>c) \<times>\<^sub>c \<nat>\<^sub>c\<^esub>)\<^sup>\<sharp> \<circ>\<^sub>c zero : (\<nat>\<^sub>c \<times>\<^sub>c \<nat>\<^sub>c) \<times>\<^sub>c one \<rightarrow> \<Omega>"
+          by typecheck_cfuncs
+        show "\<And>x. x \<in>\<^sub>c (\<nat>\<^sub>c \<times>\<^sub>c \<nat>\<^sub>c) \<times>\<^sub>c one \<Longrightarrow>
+         (eval_func \<Omega> (\<nat>\<^sub>c \<times>\<^sub>c \<nat>\<^sub>c) \<circ>\<^sub>c id\<^sub>c (\<nat>\<^sub>c \<times>\<^sub>c \<nat>\<^sub>c) \<times>\<^sub>f \<phi>\<^sup>\<sharp> \<circ>\<^sub>c zero) \<circ>\<^sub>c x =
+         (eval_func \<Omega> (\<nat>\<^sub>c \<times>\<^sub>c \<nat>\<^sub>c) \<circ>\<^sub>c id\<^sub>c (\<nat>\<^sub>c \<times>\<^sub>c \<nat>\<^sub>c) \<times>\<^sub>f (\<t> \<circ>\<^sub>c \<beta>\<^bsub>(\<nat>\<^sub>c \<times>\<^sub>c \<nat>\<^sub>c) \<times>\<^sub>c \<nat>\<^sub>c\<^esub>)\<^sup>\<sharp> \<circ>\<^sub>c zero) \<circ>\<^sub>c x"
+        proof - 
+          fix x 
+          assume x_type: "x \<in>\<^sub>c (\<nat>\<^sub>c \<times>\<^sub>c \<nat>\<^sub>c) \<times>\<^sub>c one"
+          obtain y where x_def: "y \<in>\<^sub>c (\<nat>\<^sub>c \<times>\<^sub>c \<nat>\<^sub>c) \<and>  x = \<langle>y, id(one)\<rangle>"
+            using cart_prod_decomp id_type one_unique_element x_type by blast
+          obtain m n where y_def: "m \<in>\<^sub>c \<nat>\<^sub>c \<and> n \<in>\<^sub>c \<nat>\<^sub>c \<and> y = \<langle>m,n\<rangle>"
+            using cart_prod_decomp x_def by blast
+          have m0_type: "\<langle>m,zero\<rangle> \<in>\<^sub>c (\<nat>\<^sub>c \<times>\<^sub>c \<nat>\<^sub>c)"
+            by (simp add: cfunc_prod_type y_def zero_type)
+          have n0_type: "\<langle>n,zero\<rangle> \<in>\<^sub>c (\<nat>\<^sub>c \<times>\<^sub>c \<nat>\<^sub>c)"
+            by (simp add: cfunc_prod_type y_def zero_type)
+          have m0n0_type: "\<langle>\<langle>m,zero\<rangle>, \<langle>n,zero\<rangle>\<rangle> \<in>\<^sub>c (\<nat>\<^sub>c \<times>\<^sub>c \<nat>\<^sub>c) \<times>\<^sub>c (\<nat>\<^sub>c \<times>\<^sub>c \<nat>\<^sub>c)"
+            using cfunc_prod_type m0_type n0_type by blast
+
+          have "(eval_func \<Omega> (\<nat>\<^sub>c \<times>\<^sub>c \<nat>\<^sub>c) \<circ>\<^sub>c id\<^sub>c (\<nat>\<^sub>c \<times>\<^sub>c \<nat>\<^sub>c) \<times>\<^sub>f \<phi>\<^sup>\<sharp> \<circ>\<^sub>c zero) \<circ>\<^sub>c x =
+                ((eval_func \<Omega> (\<nat>\<^sub>c \<times>\<^sub>c \<nat>\<^sub>c) \<circ>\<^sub>c id\<^sub>c (\<nat>\<^sub>c \<times>\<^sub>c \<nat>\<^sub>c) \<times>\<^sub>f \<phi>\<^sup>\<sharp>) \<circ>\<^sub>c ( id\<^sub>c (\<nat>\<^sub>c \<times>\<^sub>c \<nat>\<^sub>c) \<times>\<^sub>fzero)) \<circ>\<^sub>c x"
+            by (typecheck_cfuncs, metis \<phi>_sharp_type inv_transpose_func_def2 inv_transpose_of_composition)
+          also have "... = (\<phi> \<circ>\<^sub>c ( id\<^sub>c (\<nat>\<^sub>c \<times>\<^sub>c \<nat>\<^sub>c) \<times>\<^sub>fzero)) \<circ>\<^sub>c x"
+            using \<phi>_type transpose_func_def by auto
+          also have "... = \<phi> \<circ>\<^sub>c ( id\<^sub>c (\<nat>\<^sub>c \<times>\<^sub>c \<nat>\<^sub>c) \<times>\<^sub>fzero) \<circ>\<^sub>c x"
+            using \<phi>_type comp_associative2 x_type by (typecheck_cfuncs, auto) 
+          also have "... = \<phi> \<circ>\<^sub>c \<langle>id\<^sub>c (\<nat>\<^sub>c \<times>\<^sub>c \<nat>\<^sub>c) \<circ>\<^sub>c \<langle>m,n\<rangle>,zero \<circ>\<^sub>c id(one)\<rangle>"
+            by (typecheck_cfuncs, smt cfunc_cross_prod_comp_cfunc_prod x_def y_def)
+          also have "... = \<phi> \<circ>\<^sub>c \<langle>\<langle>m,n\<rangle>,zero\<rangle>"
+            by (typecheck_cfuncs, metis id_left_unit2 id_right_unit2 y_def)
+          also have "... = (leq \<circ>\<^sub>c (exp_uncurried \<times>\<^sub>f exp_uncurried)) \<circ>\<^sub>c ((distribute_right \<nat>\<^sub>c \<nat>\<^sub>c \<nat>\<^sub>c)\<circ>\<^sub>c \<langle>\<langle>m,n\<rangle>,zero\<rangle>)"
+            by (typecheck_cfuncs, smt \<phi>_def comp_associative2 y_def)
+          also have "... = (leq \<circ>\<^sub>c (exp_uncurried \<times>\<^sub>f exp_uncurried)) \<circ>\<^sub>c \<langle>\<langle>m,zero\<rangle>,\<langle>n,zero\<rangle>\<rangle>"
+            using distribute_right_ap y_def by (typecheck_cfuncs, auto)
+          also have "... = leq \<circ>\<^sub>c (exp_uncurried \<times>\<^sub>f exp_uncurried) \<circ>\<^sub>c \<langle>\<langle>m,zero\<rangle>,\<langle>n,zero\<rangle>\<rangle>"
+            using comp_associative2 m0n0_type by (typecheck_cfuncs, auto)
+          also have "... = leq \<circ>\<^sub>c  \<langle>exp_uncurried \<circ>\<^sub>c \<langle>m,zero\<rangle>,exp_uncurried \<circ>\<^sub>c \<langle>n,zero\<rangle>\<rangle>"
+            using cfunc_cross_prod_comp_cfunc_prod m0_type n0_type by (typecheck_cfuncs, auto)
+          also have "... = leq \<circ>\<^sub>c \<langle>m ^\<^sub>\<nat> zero, n ^\<^sub>\<nat> zero\<rangle>"
+            by (simp add: exp_def)
+          also have "... = leq \<circ>\<^sub>c \<langle>successor \<circ>\<^sub>c zero, successor \<circ>\<^sub>c zero\<rangle>"
+            by (simp add: exp_respects_Zero_Left y_def)
+          also have "... = \<t>"
+            using lqe_connexity succ_n_type zero_type by blast
+          also have "... = \<t> \<circ>\<^sub>c id(one)"
+            using id_right_unit2 true_func_type by auto
+          also have "... = \<t> \<circ>\<^sub>c (((\<beta>\<^bsub>(\<nat>\<^sub>c \<times>\<^sub>c \<nat>\<^sub>c) \<times>\<^sub>c \<nat>\<^sub>c\<^esub>) \<circ>\<^sub>c ( id\<^sub>c (\<nat>\<^sub>c \<times>\<^sub>c \<nat>\<^sub>c) \<times>\<^sub>fzero)) \<circ>\<^sub>c x)"
+            by (typecheck_cfuncs, metis terminal_func_unique x_type)
+          also have "... = ((\<t> \<circ>\<^sub>c \<beta>\<^bsub>(\<nat>\<^sub>c \<times>\<^sub>c \<nat>\<^sub>c) \<times>\<^sub>c \<nat>\<^sub>c\<^esub>) \<circ>\<^sub>c ( id\<^sub>c (\<nat>\<^sub>c \<times>\<^sub>c \<nat>\<^sub>c) \<times>\<^sub>fzero)) \<circ>\<^sub>c x"
+            using comp_associative2 x_type by (typecheck_cfuncs, auto)
+          also have "... = ((eval_func \<Omega> (\<nat>\<^sub>c \<times>\<^sub>c \<nat>\<^sub>c) \<circ>\<^sub>c id\<^sub>c (\<nat>\<^sub>c \<times>\<^sub>c \<nat>\<^sub>c) \<times>\<^sub>f (\<t> \<circ>\<^sub>c \<beta>\<^bsub>(\<nat>\<^sub>c \<times>\<^sub>c \<nat>\<^sub>c) \<times>\<^sub>c \<nat>\<^sub>c\<^esub>)\<^sup>\<sharp>) \<circ>\<^sub>c ( id\<^sub>c (\<nat>\<^sub>c \<times>\<^sub>c \<nat>\<^sub>c) \<times>\<^sub>fzero)) \<circ>\<^sub>c x"
+            by (typecheck_cfuncs, simp add: transpose_func_def)
+          also have "... = (eval_func \<Omega> (\<nat>\<^sub>c \<times>\<^sub>c \<nat>\<^sub>c) \<circ>\<^sub>c id\<^sub>c (\<nat>\<^sub>c \<times>\<^sub>c \<nat>\<^sub>c) \<times>\<^sub>f (\<t> \<circ>\<^sub>c \<beta>\<^bsub>(\<nat>\<^sub>c \<times>\<^sub>c \<nat>\<^sub>c) \<times>\<^sub>c \<nat>\<^sub>c\<^esub>)\<^sup>\<sharp> \<circ>\<^sub>c zero) \<circ>\<^sub>c x"
+            by (typecheck_cfuncs, metis inv_transpose_func_def2 inv_transpose_of_composition)
+          then show "(eval_func \<Omega> (\<nat>\<^sub>c \<times>\<^sub>c \<nat>\<^sub>c) \<circ>\<^sub>c id\<^sub>c (\<nat>\<^sub>c \<times>\<^sub>c \<nat>\<^sub>c) \<times>\<^sub>f \<phi>\<^sup>\<sharp> \<circ>\<^sub>c zero) \<circ>\<^sub>c x =
+                     (eval_func \<Omega> (\<nat>\<^sub>c \<times>\<^sub>c \<nat>\<^sub>c) \<circ>\<^sub>c id\<^sub>c (\<nat>\<^sub>c \<times>\<^sub>c \<nat>\<^sub>c) \<times>\<^sub>f (\<t> \<circ>\<^sub>c \<beta>\<^bsub>(\<nat>\<^sub>c \<times>\<^sub>c \<nat>\<^sub>c) \<times>\<^sub>c \<nat>\<^sub>c\<^esub>)\<^sup>\<sharp> \<circ>\<^sub>c zero) \<circ>\<^sub>c x"
+            by (simp add: calculation)
+        qed
+      qed
+    qed
+    show "\<phi>\<^sup>\<sharp> \<circ>\<^sub>c successor = id\<^sub>c (\<Omega>\<^bsup>(\<nat>\<^sub>c \<times>\<^sub>c \<nat>\<^sub>c)\<^esup>) \<circ>\<^sub>c \<phi>\<^sup>\<sharp>"
+    proof(rule same_evals_equal[where Z ="\<nat>\<^sub>c", where X = "\<Omega>", where A = "(\<nat>\<^sub>c \<times>\<^sub>c \<nat>\<^sub>c)"])
+      show phi_succ_type: "\<phi>\<^sup>\<sharp> \<circ>\<^sub>c successor : \<nat>\<^sub>c \<rightarrow> \<Omega>\<^bsup>(\<nat>\<^sub>c \<times>\<^sub>c \<nat>\<^sub>c)\<^esup>"
+        using \<phi>_sharp_type by typecheck_cfuncs
+      show "id\<^sub>c (\<Omega>\<^bsup>(\<nat>\<^sub>c \<times>\<^sub>c \<nat>\<^sub>c)\<^esup>) \<circ>\<^sub>c \<phi>\<^sup>\<sharp> : \<nat>\<^sub>c \<rightarrow> \<Omega>\<^bsup>(\<nat>\<^sub>c \<times>\<^sub>c \<nat>\<^sub>c)\<^esup>"
+        using \<phi>_sharp_type by typecheck_cfuncs
+      show "eval_func \<Omega> (\<nat>\<^sub>c \<times>\<^sub>c \<nat>\<^sub>c) \<circ>\<^sub>c id\<^sub>c (\<nat>\<^sub>c \<times>\<^sub>c \<nat>\<^sub>c) \<times>\<^sub>f \<phi>\<^sup>\<sharp> \<circ>\<^sub>c successor =
+            eval_func \<Omega> (\<nat>\<^sub>c \<times>\<^sub>c \<nat>\<^sub>c) \<circ>\<^sub>c id\<^sub>c (\<nat>\<^sub>c \<times>\<^sub>c \<nat>\<^sub>c) \<times>\<^sub>f id\<^sub>c (\<Omega>\<^bsup>(\<nat>\<^sub>c \<times>\<^sub>c \<nat>\<^sub>c)\<^esup>) \<circ>\<^sub>c \<phi>\<^sup>\<sharp>"
+      proof(rule one_separator[where X = "(\<nat>\<^sub>c \<times>\<^sub>c \<nat>\<^sub>c)\<times>\<^sub>c \<nat>\<^sub>c", where Y = "\<Omega>"])
+        show "eval_func \<Omega> (\<nat>\<^sub>c \<times>\<^sub>c \<nat>\<^sub>c) \<circ>\<^sub>c id\<^sub>c (\<nat>\<^sub>c \<times>\<^sub>c \<nat>\<^sub>c) \<times>\<^sub>f \<phi>\<^sup>\<sharp> \<circ>\<^sub>c successor : (\<nat>\<^sub>c \<times>\<^sub>c \<nat>\<^sub>c) \<times>\<^sub>c \<nat>\<^sub>c \<rightarrow> \<Omega>"
+          using phi_succ_type by typecheck_cfuncs
+        show "eval_func \<Omega> (\<nat>\<^sub>c \<times>\<^sub>c \<nat>\<^sub>c) \<circ>\<^sub>c id\<^sub>c (\<nat>\<^sub>c \<times>\<^sub>c \<nat>\<^sub>c) \<times>\<^sub>f id\<^sub>c (\<Omega>\<^bsup>(\<nat>\<^sub>c \<times>\<^sub>c \<nat>\<^sub>c)\<^esup>) \<circ>\<^sub>c \<phi>\<^sup>\<sharp> : (\<nat>\<^sub>c \<times>\<^sub>c \<nat>\<^sub>c) \<times>\<^sub>c \<nat>\<^sub>c \<rightarrow> \<Omega>"
+          using \<phi>_type by typecheck_cfuncs
+        show "\<And>x. x \<in>\<^sub>c (\<nat>\<^sub>c \<times>\<^sub>c \<nat>\<^sub>c) \<times>\<^sub>c \<nat>\<^sub>c \<Longrightarrow>
+         (eval_func \<Omega> (\<nat>\<^sub>c \<times>\<^sub>c \<nat>\<^sub>c) \<circ>\<^sub>c id\<^sub>c (\<nat>\<^sub>c \<times>\<^sub>c \<nat>\<^sub>c) \<times>\<^sub>f \<phi>\<^sup>\<sharp> \<circ>\<^sub>c successor) \<circ>\<^sub>c x =
+         (eval_func \<Omega> (\<nat>\<^sub>c \<times>\<^sub>c \<nat>\<^sub>c) \<circ>\<^sub>c id\<^sub>c (\<nat>\<^sub>c \<times>\<^sub>c \<nat>\<^sub>c) \<times>\<^sub>f id\<^sub>c (\<Omega>\<^bsup>(\<nat>\<^sub>c \<times>\<^sub>c \<nat>\<^sub>c)\<^esup>) \<circ>\<^sub>c \<phi>\<^sup>\<sharp>) \<circ>\<^sub>c x"
+        proof - 
+          fix x 
+          assume x_type: "x \<in>\<^sub>c (\<nat>\<^sub>c \<times>\<^sub>c \<nat>\<^sub>c) \<times>\<^sub>c \<nat>\<^sub>c"
+          obtain y p where p_def: "y \<in>\<^sub>c (\<nat>\<^sub>c \<times>\<^sub>c \<nat>\<^sub>c) \<and> p \<in>\<^sub>c \<nat>\<^sub>c \<and> x = \<langle>y,p\<rangle>"
+            using cart_prod_decomp x_type by blast
+          obtain m n where y_def: "m \<in>\<^sub>c \<nat>\<^sub>c \<and> n \<in>\<^sub>c \<nat>\<^sub>c \<and> y = \<langle>m,n\<rangle>"
+            using cart_prod_decomp p_def by blast
+          have mnsp_type: "\<langle>\<langle>m,n\<rangle>,successor \<circ>\<^sub>c p\<rangle> \<in>\<^sub>c (\<nat>\<^sub>c \<times>\<^sub>c \<nat>\<^sub>c) \<times>\<^sub>c \<nat>\<^sub>c"
+            using p_def y_def by (typecheck_cfuncs, blast)
+          have msp_type: "\<langle>m,successor \<circ>\<^sub>c p\<rangle> \<in>\<^sub>c (\<nat>\<^sub>c \<times>\<^sub>c \<nat>\<^sub>c)"
+            by (simp add: cfunc_prod_type p_def succ_n_type y_def)
+          have nsp_type: "\<langle>n,successor \<circ>\<^sub>c p\<rangle> \<in>\<^sub>c (\<nat>\<^sub>c \<times>\<^sub>c \<nat>\<^sub>c)"
+            by (simp add: cfunc_prod_type p_def succ_n_type y_def)
+          have mspnsp_type: "\<langle>\<langle>m,successor \<circ>\<^sub>c p\<rangle>,\<langle>n,successor \<circ>\<^sub>c p\<rangle>\<rangle> \<in>\<^sub>c (\<nat>\<^sub>c \<times>\<^sub>c \<nat>\<^sub>c) \<times>\<^sub>c (\<nat>\<^sub>c \<times>\<^sub>c \<nat>\<^sub>c)"
+            by (simp add: cfunc_prod_type msp_type nsp_type)
+          have mp_type: "\<langle>m,p\<rangle> \<in>\<^sub>c (\<nat>\<^sub>c \<times>\<^sub>c \<nat>\<^sub>c)"
+            by (simp add: cfunc_prod_type p_def y_def)
+          have np_type: "\<langle>n,p\<rangle> \<in>\<^sub>c (\<nat>\<^sub>c \<times>\<^sub>c \<nat>\<^sub>c)"
+            by (simp add: cfunc_prod_type p_def y_def)
+          have mpnp_type: "\<langle>\<langle>m,p\<rangle>,\<langle>n,p\<rangle>\<rangle> \<in>\<^sub>c (\<nat>\<^sub>c \<times>\<^sub>c \<nat>\<^sub>c) \<times>\<^sub>c (\<nat>\<^sub>c \<times>\<^sub>c \<nat>\<^sub>c)"
+            by (simp add: cfunc_prod_type mp_type np_type)
+
+
+
+
+          
+
+
+
+
+          have "(eval_func \<Omega> (\<nat>\<^sub>c \<times>\<^sub>c \<nat>\<^sub>c) \<circ>\<^sub>c id\<^sub>c (\<nat>\<^sub>c \<times>\<^sub>c \<nat>\<^sub>c) \<times>\<^sub>f \<phi>\<^sup>\<sharp> \<circ>\<^sub>c successor) \<circ>\<^sub>c x =
+               ((eval_func \<Omega> (\<nat>\<^sub>c \<times>\<^sub>c \<nat>\<^sub>c) \<circ>\<^sub>c id\<^sub>c (\<nat>\<^sub>c \<times>\<^sub>c \<nat>\<^sub>c) \<times>\<^sub>f \<phi>\<^sup>\<sharp>) \<circ>\<^sub>c (id\<^sub>c (\<nat>\<^sub>c \<times>\<^sub>c \<nat>\<^sub>c) \<times>\<^sub>fsuccessor)) \<circ>\<^sub>c x" 
+            by (typecheck_cfuncs, metis \<phi>_sharp_type inv_transpose_func_def2 inv_transpose_of_composition)
+          also have "... = (\<phi> \<circ>\<^sub>c (id\<^sub>c (\<nat>\<^sub>c \<times>\<^sub>c \<nat>\<^sub>c) \<times>\<^sub>fsuccessor)) \<circ>\<^sub>c x" 
+            using \<phi>_type transpose_func_def by (typecheck_cfuncs, auto)
+          also have "... = \<phi> \<circ>\<^sub>c ((id\<^sub>c (\<nat>\<^sub>c \<times>\<^sub>c \<nat>\<^sub>c) \<times>\<^sub>fsuccessor) \<circ>\<^sub>c x)"
+            using \<phi>_type comp_associative2 x_type by (typecheck_cfuncs, auto)
+          also have "... = \<phi> \<circ>\<^sub>c \<langle>id\<^sub>c (\<nat>\<^sub>c \<times>\<^sub>c \<nat>\<^sub>c) \<circ>\<^sub>c \<langle>m,n\<rangle>,successor \<circ>\<^sub>c p\<rangle>"
+            by (typecheck_cfuncs, smt cfunc_cross_prod_comp_cfunc_prod p_def y_def)
+          also have "... = \<phi> \<circ>\<^sub>c \<langle>\<langle>m,n\<rangle>,successor \<circ>\<^sub>c p\<rangle>"
+            by (typecheck_cfuncs, metis id_left_unit2 y_def)
+          also have "... = (leq \<circ>\<^sub>c (exp_uncurried \<times>\<^sub>f exp_uncurried))\<circ>\<^sub>c ((distribute_right \<nat>\<^sub>c \<nat>\<^sub>c \<nat>\<^sub>c) \<circ>\<^sub>c \<langle>\<langle>m,n\<rangle>,successor \<circ>\<^sub>c p\<rangle>)"
+            using \<phi>_def comp_associative2 mnsp_type by (typecheck_cfuncs, auto)
+          also have "... = (leq \<circ>\<^sub>c (exp_uncurried \<times>\<^sub>f exp_uncurried))\<circ>\<^sub>c  \<langle>\<langle>m,successor \<circ>\<^sub>c p\<rangle>,\<langle>n,successor \<circ>\<^sub>c p\<rangle>\<rangle>"
+            using distribute_right_ap p_def y_def by (typecheck_cfuncs, auto)
+          also have "... = leq \<circ>\<^sub>c (exp_uncurried \<times>\<^sub>f exp_uncurried)\<circ>\<^sub>c  \<langle>\<langle>m,successor \<circ>\<^sub>c p\<rangle>,\<langle>n,successor \<circ>\<^sub>c p\<rangle>\<rangle>"
+            using comp_associative2 mspnsp_type by (typecheck_cfuncs, auto) 
+          also have "... = leq \<circ>\<^sub>c \<langle>exp_uncurried \<circ>\<^sub>c \<langle>m,successor \<circ>\<^sub>c p\<rangle>,exp_uncurried \<circ>\<^sub>c \<langle>n,successor \<circ>\<^sub>c p\<rangle>\<rangle>"
+            using cfunc_cross_prod_comp_cfunc_prod msp_type nsp_type by (typecheck_cfuncs, auto)
+          also have "... = leq \<circ>\<^sub>c \<langle>m ^\<^sub>\<nat> (successor \<circ>\<^sub>c p),n ^\<^sub>\<nat> (successor \<circ>\<^sub>c p)\<rangle>"
+            by (simp add: exp_def)
+          also have "... = leq \<circ>\<^sub>c \<langle>m \<cdot>\<^sub>\<nat>(m ^\<^sub>\<nat> p),n \<cdot>\<^sub>\<nat>(n ^\<^sub>\<nat> p)\<rangle>"
+            by (simp add: exp_respects_successor p_def y_def)
+          also have "... = leq \<circ>\<^sub>c \<langle>(m ^\<^sub>\<nat> p),(n ^\<^sub>\<nat> p)\<rangle>"
+            oops
+
+
+(*
+have "(eval_func \<Omega> (\<nat>\<^sub>c \<times>\<^sub>c \<nat>\<^sub>c) \<circ>\<^sub>c id\<^sub>c (\<nat>\<^sub>c \<times>\<^sub>c \<nat>\<^sub>c) \<times>\<^sub>f id\<^sub>c (\<Omega>\<^bsup>(\<nat>\<^sub>c \<times>\<^sub>c \<nat>\<^sub>c)\<^esup>) \<circ>\<^sub>c \<phi>\<^sup>\<sharp>) \<circ>\<^sub>c x = 
+                (eval_func \<Omega> (\<nat>\<^sub>c \<times>\<^sub>c \<nat>\<^sub>c) \<circ>\<^sub>c id\<^sub>c (\<nat>\<^sub>c \<times>\<^sub>c \<nat>\<^sub>c) \<times>\<^sub>f  \<phi>\<^sup>\<sharp>) \<circ>\<^sub>c x"
+            using \<phi>_sharp_type id_left_unit2 by auto
+          also have "... = \<phi> \<circ>\<^sub>c x"
+            using \<phi>_type transpose_func_def by auto
+          also have "... = (leq \<circ>\<^sub>c (exp_uncurried \<times>\<^sub>f exp_uncurried))\<circ>\<^sub>c \<langle>\<langle>m,p\<rangle>,\<langle>n,p\<rangle>\<rangle>"
+            by (typecheck_cfuncs, smt \<phi>_def comp_associative2 distribute_right_ap distribute_right_type p_def x_type y_def)
+          also have "... = leq \<circ>\<^sub>c (exp_uncurried \<times>\<^sub>f exp_uncurried)\<circ>\<^sub>c \<langle>\<langle>m,p\<rangle>,\<langle>n,p\<rangle>\<rangle>"
+            using comp_associative2 mpnp_type by (typecheck_cfuncs, auto)
+          also have "... = leq \<circ>\<^sub>c \<langle>exp_uncurried \<circ>\<^sub>c \<langle>m,p\<rangle>,exp_uncurried \<circ>\<^sub>c \<langle>n,p\<rangle>\<rangle>"
+            using cfunc_cross_prod_comp_cfunc_prod mp_type np_type by (typecheck_cfuncs,auto)
+            by (simp add: exp_def)
+            apply typecheck_cfuncs
+            oops
 *)
+
+
+
 
 
 lemma nonzero_to_k_nonzero:
@@ -52,7 +216,7 @@ qed
 
 
 
-lemma exp_order_preserving:
+lemma exp_order_preserving2:
   assumes x_type: "x \<in>\<^sub>c \<nat>\<^sub>c" and y_type: "y \<in>\<^sub>c \<nat>\<^sub>c" and a_type: "a \<in>\<^sub>c \<nat>\<^sub>c"
   assumes a_nonzero: "a \<noteq> zero"
   assumes leq_true: "leq \<circ>\<^sub>c \<langle>x, y\<rangle> = \<t>"
@@ -91,7 +255,7 @@ lemma mult_le_exp:
   assumes "a \<noteq> successor \<circ>\<^sub>c zero" and "b \<noteq> zero"
   assumes "\<And>x y z. x \<in>\<^sub>c \<nat>\<^sub>c \<Longrightarrow>  y \<in>\<^sub>c \<nat>\<^sub>c \<Longrightarrow>  z \<in>\<^sub>c \<nat>\<^sub>c \<Longrightarrow>  leq \<circ>\<^sub>c \<langle>x , y\<rangle> = \<t>  \<Longrightarrow> leq \<circ>\<^sub>c \<langle>x ^\<^sub>\<nat> z , y ^\<^sub>\<nat> z\<rangle> = \<t>" (*Delete once above is proven*)
   assumes "\<And> n. n \<in>\<^sub>c \<nat>\<^sub>c \<Longrightarrow> leq \<circ>\<^sub>c \<langle>successor \<circ>\<^sub>c n , (successor \<circ>\<^sub>c (successor \<circ>\<^sub>c zero)) ^\<^sub>\<nat> n \<rangle> = \<t>" (*Delete once above is proven*)
-  shows "leq \<circ>\<^sub>c \<langle>a  \<cdot>\<^sub>\<nat> b , a ^\<^sub>\<nat> b\<rangle> = \<t>"
+  shows "leq \<circ>\<^sub>c \<langle>a \<cdot>\<^sub>\<nat> b , a ^\<^sub>\<nat> b\<rangle> = \<t>"
 proof(cases "a = zero",auto)
   show "a = zero \<Longrightarrow> leq \<circ>\<^sub>c \<langle>zero \<cdot>\<^sub>\<nat> b,zero ^\<^sub>\<nat> b\<rangle> = \<t>"
     by (typecheck_cfuncs, simp add: assms(2) mult_respects_zero_left zero_is_smallest)
